\documentclass{article}
\usepackage{epsfig}
\usepackage{amsmath}
\usepackage{amssymb}
\usepackage{mathrsfs}
\pagestyle{empty}
\begin{document}
\[ f(x|\theta) = \frac{1}{2 \theta}\exp\left(-\frac{\|x - \mu\|}{\theta}\right) \]
\pagebreak

$\theta$
\pagebreak

$\mu$
\pagebreak

\[ d(a, b) = \frac{a^T b}{|| a || || b ||} \]
\pagebreak

\[ K(x, y) = \max \{0, 1 - || x - y ||^2_2 / b^2 \} \]
\pagebreak

$ b $
\pagebreak

$ K(x, y) $
\pagebreak

$ x $
\pagebreak

$ y $
\pagebreak

\[ \int \int K(x, y) g(x) g(y) dx dy \ge 0 \]
\pagebreak

$ g(x) $
\pagebreak

$ \mu $
\pagebreak

\[ K(x, y) = \exp(-\frac{|| x - y ||^2}{2 \mu^2}). \]
\pagebreak

$ \gamma = -\frac{1}{2 \mu^2} $
\pagebreak

$ s $
\pagebreak

$ t $
\pagebreak

\[ K(x, y) = \tanh(s <x, y> + t) \]
\pagebreak

\[ K(x, y) = \exp(-\frac{|| x - y ||}{\mu}). \]
\pagebreak

\[ K(x, y) = x^T y \]
\pagebreak

$ degree $
\pagebreak

$ offset $
\pagebreak

\[ K(x, y) = (x^T * y + offset) ^ {degree}. \]
\pagebreak

\[ K(x, y) = \max \{ 0, 1 - \frac{|| x - y ||_2}{b} \} \]
\pagebreak

$ W = x (x^T x)^{-0.5} $
\pagebreak

\[ d(x, y) = \sqrt{ K(x, x) + K(y, y) - 2K(x, y) }. \]
\pagebreak

$ n $
\pagebreak

\[ d(x, y) = \left( \sum_{i = 1}^{n} | x_i - y_i |^p \right)^{\frac{1}{p}}. \]
\pagebreak

$ d(x, y) $
\pagebreak

\[ d(x, y) = \sum_{i = 1}^{n} | x_i - y_i |^p \]
\pagebreak

$ Q $
\pagebreak

$ d $
\pagebreak

\[ d(x, y) = \sqrt{(x - y)^T Q (x - y)} \]
\pagebreak

\[ d(x, y) = (x - y)^T Q (x - y) \]
\pagebreak

\[ T_{n+1} = (1-\lambda) T_{n} \]
\pagebreak

$ 0<\lambda<1 $
\pagebreak

$ \lambda $
\pagebreak

$ \alpha = (-1 \lambda) $
\pagebreak

$ \alpha $
\pagebreak

\[ f(A) = \sum_{i = 0}^{n} f_i(A) \]
\pagebreak

$ A $
\pagebreak

$ f_i(A) $
\pagebreak

\[ A_{j + 1} = A_j + \alpha \nabla f_i(A) \]
\pagebreak

$ i $
\pagebreak

$ j $
\pagebreak

$ \epsilon $
\pagebreak

\[ | f(A_{j + n}) - f(A_j) | < \epsilon. \]
\pagebreak

$\epsilon$
\pagebreak

$n$
\pagebreak

$ V \approx WH $
\pagebreak

$ \sqrt{\sum_i \sum_j(V-WH)^2} $
\pagebreak

\[ W^T = \frac{H V^T}{H H^T} \]
\pagebreak

\[ H = \frac{W^T V}{W^T W} \]
\pagebreak

\[ W_{ia} \leftarrow W_{ia} \frac{(VH^T)_{ia}}{(WHH^T)_{ia}} \]
\pagebreak

\[ H_{a\mu} \leftarrow H_{a\mu} \frac{(W^T V)_{a\mu}}{(W^T WH)_{a\mu}} \]
\pagebreak

\[ \sum_i \sum_j (V_{ij} \log\frac{V_{ij}}{(W H)_{ij}} - V_{ij} + (W H)_{ij}) \]
\pagebreak

\[ W_{ia} \leftarrow W_{ia} \frac{\sum_{\mu} H_{a\mu} V_{i\mu} / (W H)_{i\mu}} {\sum_{\nu} H_{a\nu}} \]
\pagebreak

\[ H_{a\mu} \leftarrow H_{a\mu} \frac{\sum_{i} W_{ia} V_{i\mu}/(WH)_{i\mu}} {\sum_{k} H_{ka}} \]
\pagebreak

\[ \min_{\beta} 0.5 || X \beta - y ||_2^2 + 0.5 \lambda_2 || \beta ||_2^2 \]
\pagebreak

$ ||\beta||_1 <= \tau $
\pagebreak

$ X $
\pagebreak

\[ \min_{\beta} 0.5 || X \beta - y ||_2^2 + \lambda_1 || \beta ||_1 + 0.5 \lambda_2 || \beta ||_2^2 \]
\pagebreak

$ \beta $
\pagebreak

$ \lambda_1 > 0 $
\pagebreak

$ \lambda_2 = 0 $
\pagebreak

$ \lambda_2 > 0 $
\pagebreak

$ \lambda_1 = 0 $
\pagebreak

$ \lambda_1 $
\pagebreak

\[ (1 / n) * \| y - X B \|^2_2 \]
\pagebreak

$ B $
\pagebreak

\[ \min_{D,Z} 0.5 ||X - D Z||_{F}^2\ + \lambda_1 \sum_{i=1}^m ||Z_i||_1 + 0.5 \lambda_2 \sum_{i=1}^m ||Z_i||_2^2 \]
\pagebreak

$ ||D_j||_2 <= 1 $
\pagebreak

$ 1 <= j <= k $
\pagebreak

$ lambda_1 > 0 $
\pagebreak

$ lambda_2 = 0 $
\pagebreak

$ C = X^T X $
\pagebreak

$ C = X X^T $
\pagebreak

$m$
\pagebreak

$V \in \Re^{n \times m}$
\pagebreak

$V_{ij}$
\pagebreak

$i$
\pagebreak

$j$
\pagebreak

$V$
\pagebreak

$V \approx WH$
\pagebreak

$W$
\pagebreak

$H$
\pagebreak

$\alpha$
\pagebreak

$S$
\pagebreak

$\mathbf{R}^d$
\pagebreak

$kd$
\pagebreak

$n-1 \times 3 $
\pagebreak

$\log N$
\pagebreak

$N$
\pagebreak

$O(N^2)$
\pagebreak

$Q$
\pagebreak

$R$
\pagebreak

\[ \arg\max_{p_r \in R} K(p_q, p_r) \]
\pagebreak

$p_q \in Q$
\pagebreak

$K(\cdot, \cdot)$
\pagebreak

$ x_i $
\pagebreak

$ c_j $
\pagebreak

$ j \le k $
\pagebreak

$ k $
\pagebreak

\[ \sum_{j = 1}^{k} \sum_{x_i \in c_j} \| x_i - \mu_j \|^2 \]
\pagebreak

$\mu_j$
\pagebreak

$c_j$
\pagebreak

$x_i$
\pagebreak

$X$
\pagebreak

$O(kN)$
\pagebreak

$\mathbf{x_i}, 0 \le i < n$
\pagebreak

$d$
\pagebreak

$y_i, 0 \le i < n$
\pagebreak

$\beta_i, 0 \le i \le d$
\pagebreak

\[ y_i = \beta_0 + \displaystyle\sum_{j = 1}^{d} \beta_j x_{ij} \]
\pagebreak

$\mathbf{x_i}$
\pagebreak

$y_i$
\pagebreak

$\mathbf{X}$
\pagebreak

$\mathbf{y}$
\pagebreak

\[ \mathbf{y} = \mathbf{X} \mathbf{\beta} + \beta_0 \]
\pagebreak

$\mathbf{\beta}$
\pagebreak

$\beta_0$
\pagebreak

$\beta_1$
\pagebreak

$\beta_2$
\pagebreak

$y$
\pagebreak

$f(y)=0+1x_1$
\pagebreak

$x_1$
\pagebreak

\[ \mathbf{X}' \mathbf{X} \]
\pagebreak

\[ \mathbf{X}' \mathbf{X} + \lambda \mathbf{I} \]
\pagebreak

$\mathbf{I}$
\pagebreak

$\lambda$
\pagebreak

$k$
\pagebreak

$\mathcal{K}(\cdot, \cdot)$
\pagebreak

$\mathcal{K}(a, b)$
\pagebreak

$ K(x, x) = 1 \; \forall x $
\pagebreak

$d(\cdot, \cdot)$
\pagebreak

$d(a, b)$
\pagebreak

$ S \in \mathcal{R}^{N \times d} $
\pagebreak

$\mathcal{R}^d$
\pagebreak

$c$
\pagebreak

$p$
\pagebreak

$d(p, c) - \lambda$
\pagebreak

\end{document}
